Micro_Rust_Std_Lib/StdLib_Range.thy
@@ -10,7 +10,8 @@ begin
 definition is_empty_contract :: \<open>'a::{ord} range \<Rightarrow> ('machine::{sepalg}, bool, 'abort) function_contract\<close> where
   [crush_contracts]: \<open>is_empty_contract r \<equiv>
     let pre  = \<top>;
-        post = \<lambda>res. \<langle>res \<longleftrightarrow> \<not>start r < end r\<rangle>
+        post = \<lambda>res. \<langle>res \<longleftrightarrow>
+          (if end_inclusive r then start r > end r else \<not>start r < end r)\<rangle>
      in make_function_contract pre post\<close>
 ucincl_auto is_empty_contract
 
@@ -21,7 +22,8 @@ by (contract f: is_empty_def contract: is_empty_contract_def) crush_base
 definition contains_contract :: \<open>'a::{ord} range \<Rightarrow> 'a \<Rightarrow> ('machine::{sepalg}, bool, 'abort) function_contract\<close> where
   [crush_contracts]: \<open>contains_contract r e \<equiv>
     let pre  = \<top>;
-        post = \<lambda>res. \<langle>res \<longleftrightarrow> start r \<le> e \<and> e < end r\<rangle>
+        post = \<lambda>res. \<langle>res \<longleftrightarrow>
+          (if end_inclusive r then start r \<le> e \<and> e \<le> end r else start r \<le> e \<and> e < end r)\<rangle>
      in make_function_contract pre post\<close>
 ucincl_auto contains_contract
 
@@ -30,7 +32,9 @@ lemma contains_spec [crush_specs]:
 by (contract f: contains_def contract: contains_contract_def) crush_base
 
 lemma range_into_list_make_range [micro_rust_simps]:
-  shows \<open>range_into_list (make_range s e) = list.map word_of_nat [unat s..<unat e]\<close>
+  shows \<open>range_into_list (make_range s e incl) =
+    (if incl then list.map word_of_nat [unat s..<Suc (unat e)]
+     else list.map word_of_nat [unat s..<unat e])\<close>
 by (clarsimp simp add: range_into_list_def)
 
 (*<*)
